tweak representation of TLB consistency in instructions
now there's just one STR, and it lets you prove TLB consistency if you
know the addr isn't in the page table, but if you don't care, you
don't have to

verified/ARMdef.s.dfy
@@ -764,29 +764,43 @@ predicate WellformedAbsPTE(pte: Maybe<AbsPTE>)
     pte.Just? ==> PageAligned(pte.v.phys) && isUInt32(pte.v.phys + PhysBase())
 }
 
+function ExtractAbsPageTable'(m:memstate, ttbr:TTBR): Maybe<AbsPTable>
+    requires ValidMemState(m)
+    ensures var r := ExtractAbsPageTable'(m, ttbr);
+        r.Just? ==> WellformedAbsPTable(fromJust(r))
+{
+    var vbase := ttbr.ptbase + PhysBase();
+    if ValidAbsL1PTable(m, vbase) then
+        Just(ExtractAbsL1PTable(m, vbase))
+    else
+        Nothing
+}
+
 function ExtractAbsPageTable(s:state): Maybe<AbsPTable>
     requires ValidState(s)
     ensures var r := ExtractAbsPageTable(s);
         r.Just? ==> WellformedAbsPTable(fromJust(r))
 {
-    var vbase := s.conf.ttbr0.ptbase + PhysBase();
-    if ValidAbsL1PTable(s.m, vbase) then
-        Just(ExtractAbsL1PTable(s.m, vbase))
-    else
-        Nothing
+    ExtractAbsPageTable'(s.m, s.conf.ttbr0)
 }
 
 // is a given address somewhere within a L1 or L2 page table, so a
 // store to it might affect TLB consistency?
+predicate AddrInPageTable'(m:memstate, ttbr:TTBR, a:addr)
+    requires ValidMemState(m)
+{
+    var pt := ExtractAbsPageTable'(m, ttbr);
+    if pt.Nothing? then true // we don't know, so be conservative
+    else
+        var vbase := ttbr.ptbase + PhysBase();
+        (vbase <= a < vbase + ARM_L1PTABLE_BYTES) // in L1
+        || AddrInL2PageTable(m, vbase, a)
+}
+
 predicate AddrInPageTable(s:state, a:addr)
     requires ValidState(s)
 {
-    var pt := ExtractAbsPageTable(s);
-    if pt.Nothing? then true // we don't know, so be conservative
-    else
-        var vbase := s.conf.ttbr0.ptbase + PhysBase();
-        (vbase <= a < vbase + ARM_L1PTABLE_BYTES) // in L1
-        || AddrInL2PageTable(s.m, vbase, a)
+    AddrInPageTable'(s.m, s.conf.ttbr0, a)
 }
 
 predicate AddrInL2PageTable(m:memstate, vbase:int, a:addr)
